pcuic/theories/PCUICOnFreeVars.v
@@ -1,0 +1,1183 @@
+(* Distributed under the terms of the MIT license. *)
+From Coq Require Import Morphisms.
+Require Import ssreflect ssrfun ssrbool.
+From MetaCoq.Template Require Import config utils MCPred.
+From MetaCoq.PCUIC Require Import PCUICAst PCUICAstUtils PCUICCases PCUICInduction
+  PCUICLiftSubst PCUICUnivSubst
+  PCUICTyping PCUICClosed PCUICEquality PCUICWeakeningEnv
+  PCUICSigmaCalculus PCUICClosed.
+
+From Equations Require Import Equations.
+Require Import Equations.Prop.DepElim.
+Set Equations With UIP.
+
+(** * Type preservation for σ-calculus operations *)
+
+Open Scope sigma_scope.
+Set Keyed Unification.
+
+Set Default Goal Selector "!".
+
+Implicit Type (cf : checker_flags).
+
+Definition shiftnP k p i :=
+  if i <? k then true else p (i - k).
+
+Instance shiftnP_ext k : Proper (`=1` ==> `=1`) (shiftnP k).
+Proof. intros f g Hfg i. now rewrite /shiftnP Hfg. Qed. 
+
+Lemma shiftnP0 P : shiftnP 0 P =1 P.
+Proof. rewrite /shiftnP. intros i; rewrite Nat.sub_0_r //. Qed.
+  
+Lemma shiftnP_add n k P : shiftnP n (shiftnP k P) =1 shiftnP (n + k) P.
+Proof. rewrite /shiftnP. intros i; repeat nat_compare_specs => //. lia_f_equal. Qed.
+
+Lemma shiftnP_impl (p q : nat -> bool) : (forall i, p i -> q i) ->
+  forall n i, shiftnP n p i -> shiftnP n q i.
+Proof.
+  intros Hi n i. rewrite /shiftnP.
+  nat_compare_specs => //. apply Hi.
+Qed.
+
+Fixpoint on_free_vars (p : nat -> bool) (t : term) : bool :=
+  match t with
+  | tRel i => p i
+  | tEvar ev args => List.forallb (on_free_vars p) args
+  | tLambda _ T M | tProd _ T M => on_free_vars p T && on_free_vars (shiftnP 1 p) M
+  | tApp u v => on_free_vars p u && on_free_vars p v
+  | tLetIn na b t b' => [&& on_free_vars p b, on_free_vars p t & on_free_vars (shiftnP 1 p) b']
+  | tCase ind pred c brs =>
+    [&& forallb (on_free_vars p) pred.(pparams),
+      on_free_vars (shiftnP #|pred.(pcontext)| p) pred.(preturn),
+      on_free_vars p c &
+      forallb (fun br => on_free_vars (shiftnP #|br.(bcontext)| p) br.(bbody)) brs]
+  | tProj _ c => on_free_vars p c
+  | tFix mfix idx | tCoFix mfix idx =>
+    List.forallb (test_def (on_free_vars p) (on_free_vars (shiftnP #|mfix| p))) mfix
+  | tVar _ | tSort _ | tConst _ _ | tInd _ _ | tConstruct _ _ _ 
+  | tPrim _ => true
+  end.
+
+Lemma on_free_vars_ext (p q : nat -> bool) t : 
+  p =1 q ->
+  on_free_vars p t = on_free_vars q t.
+Proof.
+  revert p q.
+  induction t using PCUICInduction.term_forall_list_ind; simpl => //; intros;
+    unfold test_def;
+    rewrite ?forallb_map; try eapply All_forallb_eq_forallb; tea; eauto 2.
+  all: try now rewrite (IHt1 p q) // ?(IHt2 (shiftnP 1 p) (shiftnP 1 q)) // H.
+  - now rewrite (IHt1 p q) // ?(IHt2 p q) // (IHt3 (shiftnP 1 p) (shiftnP 1 q)) // H.
+  - rewrite (IHt1 p q) // (IHt2 p q) //.
+  - destruct X. red in X0.
+    f_equal.
+    * eapply All_forallb_eq_forallb; tea. solve_all.
+    * f_equal; [eapply e; rewrite H //|].
+      f_equal; [eapply IHt; rewrite H //|].
+      eapply All_forallb_eq_forallb; tea. intros.
+      eapply H0; rewrite H //.
+  - simpl; intuition auto. f_equal; eauto 2.
+    eapply b; rewrite H //.
+  - simpl; intuition auto. f_equal; eauto 2.
+    eapply b; rewrite H //.
+Qed.
+
+Instance on_free_vars_proper : Proper (`=1` ==> Logic.eq ==> Logic.eq) on_free_vars.
+Proof. intros f g Hfg ? ? ->. now apply on_free_vars_ext. Qed.
+
+Instance on_free_vars_proper_pointwise : Proper (`=1` ==> `=1`) on_free_vars.
+Proof. intros f g Hfg x. now apply on_free_vars_ext. Qed.
+
+Lemma on_free_vars_impl (p q : nat -> bool) t : (forall i, p i -> q i) -> 
+  on_free_vars p t -> on_free_vars q t.
+Proof.
+  revert t p q.
+  induction t using PCUICInduction.term_forall_list_ind; simpl => //; solve_all.
+  all:try (rtoProp; now rewrite ?IHt1 ?IHt2 ?IHt3; eauto 2).
+  - rtoProp. intuition auto.
+    * eapply IHt1; eauto.
+    * eapply IHt2; eauto using shiftnP_impl.
+  - rtoProp; intuition auto.
+    * eapply IHt1; eauto.
+    * eapply IHt2; eauto using shiftnP_impl.
+  - rtoProp; intuition eauto 3 using shiftnP_impl.
+  - rtoProp; intuition eauto 3 using shiftnP_impl.
+    * solve_all.
+    * solve_all; eauto using shiftnP_impl.
+  - unfold test_def in *. apply /andP. move/andP: b. intuition eauto using shiftnP_impl.
+  - unfold test_def in *. apply /andP. move/andP: b. intuition eauto using shiftnP_impl.
+Qed.
+
+Definition closedP (n : nat) (P : nat -> bool) := 
+  fun i => if i <? n then P i else false.
+  
+Instance closedP_proper n : Proper (`=1` ==> `=1`) (closedP n).
+Proof. intros f g Hfg. intros i; rewrite /closedP. now rewrite Hfg. Qed.
+  
+Lemma shiftnP_closedP k n P : shiftnP k (closedP n P) =1 closedP (k + n) (shiftnP k P).
+Proof.
+  intros i; rewrite /shiftnP /closedP.
+  repeat nat_compare_specs => //.
+Qed.
+
+Lemma shiftnP_xpredT n : shiftnP n xpredT =1 xpredT.
+Proof. intros i; rewrite /shiftnP. nat_compare_specs => //. Qed.
+
+Lemma closedP_on_free_vars {n t} : closedn n t -> on_free_vars (closedP n xpredT) t.
+Proof.
+  revert n t.
+  apply: term_closedn_list_ind; simpl => //; intros.
+  all:(rewrite ?shiftnP_closedP ?shiftnP_xpredT).
+  all:try (rtoProp; now rewrite ?IHt1 ?IHt2 ?IHt3).
+  - rewrite /closedP /=. now nat_compare_specs.
+  - solve_all.
+  - destruct X. rtoProp. intuition solve_all.
+    now rewrite shiftnP_closedP shiftnP_xpredT.
+  - unfold test_def. solve_all.
+    rewrite a. rewrite shiftnP_closedP shiftnP_xpredT.
+    now len in b.
+  - unfold test_def; solve_all. 
+    rewrite a. rewrite shiftnP_closedP shiftnP_xpredT.
+    now len in b.
+Qed.
+
+Lemma closedn_on_free_vars {P n t} : closedn n t -> on_free_vars (shiftnP n P) t.
+Proof.
+  move/closedP_on_free_vars.
+  eapply on_free_vars_impl.
+  intros i; rewrite /closedP /shiftnP /= //.
+  nat_compare_specs => //.
+Qed.
+
+(** Any predicate is admissible as there are no free variables to consider *)
+Lemma closed_on_free_vars {P t} : closed t -> on_free_vars P t.
+Proof.
+  move/closedP_on_free_vars.
+  eapply on_free_vars_impl.
+  intros i; rewrite /closedP /= //.
+Qed.
+
+Lemma on_free_vars_subst_instance {p u t} : on_free_vars p t = on_free_vars p (subst_instance_constr u t).
+Proof.
+  revert t p.
+  apply: term_forall_list_ind; simpl => //; intros.
+  all:try (rtoProp; now rewrite -?IHt1 -?IHt2 -?IHt3).
+  - rewrite forallb_map. eapply All_forallb_eq_forallb; eauto.
+  - destruct X. f_equal.
+    * rewrite forallb_map; eapply All_forallb_eq_forallb; eauto.
+    * rewrite -e -H. f_equal. f_equal.
+      rewrite forallb_map. eapply All_forallb_eq_forallb; eauto.
+  - unfold test_def. rewrite forallb_map; len.
+    eapply All_forallb_eq_forallb; intuition eauto. solve_all.
+  - unfold test_def; rewrite forallb_map; len.
+    eapply All_forallb_eq_forallb; intuition eauto. solve_all.
+Qed.
+
+Definition on_free_vars_decl P d :=
+  test_decl (on_free_vars P) d.
+
+Instance on_free_vars_decl_proper : Proper (`=1` ==> Logic.eq ==> Logic.eq) on_free_vars_decl.
+Proof. rewrite /on_free_vars_decl => f g Hfg x y <-. now rewrite Hfg. Qed.
+
+Instance on_free_vars_decl_proper_pointwise : Proper (`=1` ==> `=1`) on_free_vars_decl.
+Proof. rewrite /on_free_vars_decl => f g Hfg x. now rewrite Hfg. Qed.
+
+Definition on_free_vars_ctx P ctx :=
+  alli (fun k => (on_free_vars_decl (shiftnP k P))) 0 (List.rev ctx).
+
+Instance on_free_vars_ctx_proper : Proper (`=1` ==> `=1`) on_free_vars_ctx.
+Proof.
+  rewrite /on_free_vars_ctx => f g Hfg x.
+  now setoid_rewrite Hfg. 
+Qed.
+
+Lemma on_free_vars_decl_impl (p q : nat -> bool) d : 
+  (forall i, p i -> q i) -> 
+  on_free_vars_decl p d -> on_free_vars_decl q d.
+Proof.
+  intros hpi.
+  apply test_decl_impl. intros t.
+  now apply on_free_vars_impl.
+Qed.
+
+Lemma on_free_vars_ctx_impl (p q : nat -> bool) ctx : 
+  (forall i, p i -> q i) -> 
+  on_free_vars_ctx p ctx -> on_free_vars_ctx q ctx.
+Proof.
+  intros hpi.
+  eapply alli_impl => i x.
+  apply on_free_vars_decl_impl.
+  intros k; rewrite /shiftnP.
+  now nat_compare_specs.
+Qed.
+
+Lemma closed_decl_on_free_vars {n d} : closed_decl n d -> on_free_vars_decl (closedP n xpredT) d.
+Proof.
+  rewrite /closed_decl /on_free_vars_decl /test_decl.
+  rewrite andb_comm => /andP [cld clb].
+  rewrite (closedP_on_free_vars cld) /=.
+  destruct (decl_body d) eqn:db => /= //.
+  rewrite /foroptb /=.
+  now rewrite (closedP_on_free_vars clb).
+Qed.
+
+Lemma closedn_ctx_on_free_vars {n ctx} : closedn_ctx n ctx ->
+  on_free_vars_ctx (closedP n xpredT) ctx.
+Proof.
+  rewrite /closedn_ctx /on_free_vars_ctx.
+  apply alli_impl => i x.
+  rewrite shiftnP_closedP Nat.add_comm shiftnP_xpredT.
+  eapply closed_decl_on_free_vars.
+Qed.
+
+(** This uses absurdity elimination as [ctx] can't have any free variable *)
+Lemma closed_ctx_on_free_vars P ctx : closed_ctx ctx ->
+  on_free_vars_ctx P ctx.
+Proof.
+  move/closedn_ctx_on_free_vars => /=.
+  rewrite /closedP /=.
+  eapply on_free_vars_ctx_impl => //.
+Qed.
+
+Definition nocc_betweenp k n i :=
+  (i <? k) || (k + n <=? i).
+
+Definition nocc_between k n t := 
+  (on_free_vars (nocc_betweenp k n) t).
+
+Definition noccur_shift p k := fun i => (i <? k) || p (i - k).
+
+Hint Resolve All_forallb_eq_forallb : all.
+
+Definition strengthenP k n (p : nat -> bool) := 
+  fun i => if i <? k then p i else 
+    if i <? k + n then false 
+    else p (i - n).
+
+Instance strengthenP_proper n k : Proper (`=1` ==> `=1`) (strengthenP n k).
+Proof.
+  intros f g Hfg i. rewrite /strengthenP. now rewrite (Hfg i) (Hfg (i - k)).
+Qed.
+
+Lemma shiftnP_strengthenP k' k n p : 
+  shiftnP k' (strengthenP k n p) =1 strengthenP (k' + k) n (shiftnP k' p).
+Proof.
+  intros i. rewrite /shiftnP /strengthenP.
+  repeat nat_compare_specs => /= //. 
+  lia_f_equal.
+Qed.
+
+Lemma on_free_vars_lift (p : nat -> bool) n k t : 
+  on_free_vars (strengthenP k n p) (lift n k t) = on_free_vars p t.
+Proof.
+  intros. revert t n k p.
+  induction t using PCUICInduction.term_forall_list_ind; simpl => //; intros;
+    rewrite ?forallb_map; try eapply All_forallb_eq_forallb; tea; simpl.
+  2-6:try now rewrite ?shiftnP_strengthenP ?IHt1 ?IHt2 ?IHt3.
+  - rename n0 into i. rewrite /strengthenP.
+    repeat nat_compare_specs => //.
+    lia_f_equal.
+  - intros. destruct X. red in X0.
+    rewrite !shiftnP_strengthenP e IHt.
+    f_equal.
+    + solve_all.
+    + f_equal; f_equal.
+      eapply All_forallb_eq_forallb; tea. simpl; intros.
+      now rewrite shiftnP_strengthenP.
+  - unfold test_def in *. simpl; intros ? [].
+    len; rewrite shiftnP_strengthenP. f_equal; eauto.
+  - unfold test_def in *. simpl; intros ? [].
+    len; rewrite shiftnP_strengthenP. f_equal; eauto.
+Qed.
+
+Definition on_free_vars_terms p s :=
+  forallb (on_free_vars p) s.
+  
+Definition substP (k : nat) n (q p : nat -> bool) : nat -> bool :=
+  fun i => 
+    if i <? k then p i
+    else p (i + n) || strengthenP 0 k q i.
+
+Lemma shiftnP_substP k' k n q p : 
+  shiftnP k' (substP k n q p) =1 substP (k' + k) n q (shiftnP k' p).
+Proof.
+  intros i; rewrite /shiftnP /substP.
+  repeat nat_compare_specs => //.
+  f_equal; [f_equal|].
+  * lia_f_equal.
+  * rewrite /strengthenP. simpl.
+    repeat nat_compare_specs => //.
+    lia_f_equal.
+Qed.
+
+Lemma on_free_vars_subst_gen (p q : nat -> bool) s k t : 
+  on_free_vars_terms q s ->
+  on_free_vars p t ->
+  on_free_vars (substP k #|s| q p) (subst s k t).
+Proof.
+  revert t p k.
+  induction t using PCUICInduction.term_forall_list_ind; simpl => //; intros;
+    simpl.
+  all:try (rtoProp; rewrite ?shiftnP_substP; now rewrite ?IHt1 ?IHt2 ?IHt3). 
+  - intros. destruct (Nat.leb_spec k n).
+    * destruct nth_error eqn:eq.
+      + unfold on_free_vars_terms in *. toAll.
+        pose proof (nth_error_Some_length eq).
+        eapply nth_error_all in eq; eauto.
+        simpl in eq. rewrite /substP.
+        eapply on_free_vars_impl. 
+        2:now rewrite -> on_free_vars_lift.
+        rewrite /strengthenP. simpl.
+        intros i. nat_compare_specs => //.
+        intros ->. now rewrite orb_true_r.
+      + eapply nth_error_None in eq.
+        simpl. rewrite /substP.
+        replace (n - #|s| + #|s|) with n by lia.
+        nat_compare_specs.
+        now rewrite H0.
+    * simpl. rewrite /substP /strengthenP /=.
+      rewrite H0. now nat_compare_specs.
+  - solve_all.
+  - rtoProp. destruct X. solve_all.
+    * rewrite shiftnP_substP. solve_all.
+    * rewrite shiftnP_substP; solve_all.
+  - unfold test_def in *; red in X; solve_all.
+    rtoProp. rewrite shiftnP_substP; len. solve_all.
+  - unfold test_def in *; solve_all. rtoProp.
+    rewrite shiftnP_substP; len. solve_all.
+Qed.
+
+Lemma rshiftk_S x f : S (rshiftk x f) = rshiftk (S x) f.
+Proof. reflexivity. Qed.
+
+Lemma substP_shiftnP n p : 
+  substP 0 n p (shiftnP n p) =1 p.
+Proof.
+  intros i; rewrite /shiftnP /substP /= /strengthenP /=.
+  nat_compare_specs.
+  replace (i + n - n) with i by lia.
+  now rewrite Nat.sub_0_r orb_diag.
+Qed.
+
+Lemma on_free_vars_subst (p : nat -> bool) s t : 
+  forallb (on_free_vars p) s ->
+  on_free_vars (shiftnP #|s| p) t ->
+  on_free_vars p (subst s 0 t).
+Proof.
+  intros hs ht.
+  epose proof (on_free_vars_subst_gen (shiftnP #|s| p) p s 0 t).
+  rewrite -> substP_shiftnP in H.
+  apply H.
+  - exact hs.
+  - apply ht.
+Qed.
+
+Lemma on_free_vars_subst1 (p : nat -> bool) s t : 
+  on_free_vars p s ->
+  on_free_vars (shiftnP 1 p) t ->
+  on_free_vars p (subst1 s 0 t).
+Proof.
+  intros hs ht.
+  rewrite /subst1.
+  epose proof (on_free_vars_subst_gen (shiftnP 1 p) p [s] 0 t).
+  rewrite -> substP_shiftnP in H.
+  apply H.
+  - now rewrite /on_free_vars_terms /= hs.
+  - apply ht.
+Qed.
+
+Definition addnP n (p : nat -> bool) :=
+  fun i => p (i + n).
+
+Instance addnP_proper n : Proper (`=1` ==> Logic.eq ==> Logic.eq) (addnP n).
+Proof.
+  intros i f g Hfg; now rewrite /addnP.
+Qed.
+  
+Instance addnP_proper_pointwise : Proper (Logic.eq ==> `=1` ==> `=1`) addnP.
+Proof.
+  intros i f g Hfg; now rewrite /addnP.
+Qed.
+
+Lemma addnP_add n k p : addnP n (addnP k p) =1 addnP (n + k) p.
+Proof.
+  rewrite /addnP => i. lia_f_equal.
+Qed.
+
+Lemma addnP0 p : addnP 0 p =1 p.
+Proof. intros i; now rewrite /addnP Nat.add_0_r. Qed.
+
+Lemma addnP_shiftnP n P : addnP n (shiftnP n P) =1 P.
+Proof.
+  intros i; rewrite /addnP /shiftnP /=.
+  nat_compare_specs. lia_f_equal.
+Qed.
+
+Lemma addnP_orP n p q : addnP n (predU p q) =1 predU (addnP n p) (addnP n q).
+Proof. reflexivity. Qed.
+
+Definition on_ctx_free_vars P ctx :=
+  alli (fun k d => P k ==> (on_free_vars_decl (addnP (S k) P) d)) 0 ctx.
+
+Instance on_ctx_free_vars_proper : Proper (`=1` ==> eq ==> eq) on_ctx_free_vars.
+Proof.
+  rewrite /on_ctx_free_vars => f g Hfg x y <-.
+  apply alli_ext => k.
+  now setoid_rewrite Hfg. 
+Qed.
+
+Instance on_ctx_free_vars_proper_pointwise : Proper (`=1` ==> `=1`) on_ctx_free_vars.
+Proof.
+  rewrite /on_ctx_free_vars => f g Hfg x.
+  apply alli_ext => k.
+  now setoid_rewrite Hfg. 
+Qed.
+
+Lemma nth_error_on_free_vars_ctx P n ctx i d :
+  on_ctx_free_vars (addnP n P) ctx ->
+  P (n + i) ->
+  nth_error ctx i = Some d ->
+  test_decl (on_free_vars (addnP (n + S i) P)) d.
+Proof.
+  rewrite /on_ctx_free_vars.
+  solve_all.
+  eapply alli_Alli, Alli_nth_error in H; eauto.
+  rewrite /= {1}/addnP Nat.add_comm H0 /= in H.
+  now rewrite Nat.add_comm -addnP_add.
+Qed.
+
+Definition aboveP k (p : nat -> bool) :=
+  fun i => if i <? k then false else p i.
+
+Lemma strengthenP_addn i p : strengthenP 0 i (addnP i p) =1 aboveP i p.
+Proof.
+   intros k.
+   rewrite /strengthenP /= /addnP /aboveP.
+   nat_compare_specs => //.
+   lia_f_equal.
+Qed.
+
+Lemma on_free_vars_lift0 i p t :
+  on_free_vars (addnP i p) t ->
+  on_free_vars p (lift0 i t).
+Proof.
+  rewrite -(on_free_vars_lift _ i 0).
+  rewrite /strengthenP /= /aboveP /addnP.
+  unshelve eapply on_free_vars_impl.
+  simpl. intros i'. nat_compare_specs => //.
+  now replace (i' - i + i) with i' by lia.
+Qed.
+
+Lemma on_free_vars_lift0_above i p t :
+  on_free_vars (addnP i p) t = on_free_vars (aboveP i p) (lift0 i t).
+Proof.
+  rewrite -(on_free_vars_lift _ i 0).
+  rewrite /strengthenP /= /aboveP /addnP.
+  unshelve eapply on_free_vars_ext.
+  simpl. intros i'. nat_compare_specs => //.
+  now replace (i' - i + i) with i' by lia.
+Qed.
+
+Lemma on_free_vars_mkApps p f args : 
+  on_free_vars p (mkApps f args) = on_free_vars p f && forallb (on_free_vars p) args.
+Proof.
+  induction args in f |- * => /=.
+  - now rewrite andb_true_r.
+  - now rewrite IHargs /= andb_assoc.
+Qed.
+
+Lemma extended_subst_shiftn p ctx n k : 
+  forallb (on_free_vars (strengthenP 0 n (shiftnP (k + context_assumptions ctx) p))) 
+    (extended_subst ctx (n + k)) =
+  forallb (on_free_vars (shiftnP (k + (context_assumptions ctx)) p)) 
+    (extended_subst ctx k).
+Proof.
+  rewrite lift_extended_subst' forallb_map.
+  eapply forallb_ext => t.
+  rewrite -(on_free_vars_lift _ n 0 t) //.
+Qed.
+
+Lemma extended_subst_shiftn_aboveP p ctx n k : 
+  forallb (on_free_vars (aboveP n p)) (extended_subst ctx (n + k)) =
+  forallb (on_free_vars (addnP n p)) (extended_subst ctx k).
+Proof.
+  rewrite lift_extended_subst' forallb_map.
+  eapply forallb_ext => t.
+  rewrite -(on_free_vars_lift0_above) //.
+Qed.
+
+Lemma extended_subst_shiftn_impl p ctx n k : 
+  forallb (on_free_vars (shiftnP (k + (context_assumptions ctx)) p)) 
+    (extended_subst ctx k) ->
+  forallb (on_free_vars (shiftnP (n + k + context_assumptions ctx) p))
+    (extended_subst ctx (n + k)).
+Proof.
+  rewrite lift_extended_subst' forallb_map.
+  eapply forallb_impl => t _.
+  rewrite -(on_free_vars_lift _ n 0 t).
+  rewrite /strengthenP /=.
+  apply on_free_vars_impl => i.
+  rewrite /shiftnP.
+  repeat nat_compare_specs => //.
+  intros.
+  red; rewrite -H2. lia_f_equal.
+Qed.
+
+Definition occ_betweenP k n :=
+  fun i => (k <=? i) && (i <? k + n).
+
+Lemma on_free_vars_decl_all_term P d s :
+  on_free_vars_decl P d = on_free_vars P (mkProd_or_LetIn d (tSort s)).
+Proof.
+  rewrite /on_free_vars_decl /= /test_decl.
+  destruct d as [na [b|] ty] => /= //. rewrite /foroptb /= ?andb_true_r; bool_congr.
+Qed.
+
+Lemma on_free_vars_mkProd_or_LetIn P d t :
+  on_free_vars P (mkProd_or_LetIn d t) = 
+  on_free_vars_decl P d && on_free_vars (shiftnP 1 P) t.
+Proof.
+  destruct d as [na [b|] ty]; rewrite /mkProd_or_LetIn /on_free_vars_decl /test_decl /=
+    ?andb_assoc /foroptb /=; try bool_congr.
+  f_equal. bool_congr.
+Qed.
+
+Lemma on_free_vars_ctx_all_term P ctx s :
+  on_free_vars_ctx P ctx = on_free_vars P (it_mkProd_or_LetIn ctx (tSort s)).
+Proof.
+  rewrite /on_free_vars_ctx.
+  rewrite -{2}[P](shiftnP0 P).
+  generalize 0 as k.
+  induction ctx using rev_ind; simpl; auto; intros k.
+  rewrite List.rev_app_distr alli_app /= andb_true_r.
+  rewrite IHctx it_mkProd_or_LetIn_app /= on_free_vars_mkProd_or_LetIn.
+  now rewrite shiftnP_add.
+Qed.
+
+Definition on_free_vars_ctx_k P n ctx :=
+  alli (fun k => (on_free_vars_decl (shiftnP k P))) n (List.rev ctx).
+
+Definition predA {A} (p q : pred A) : simpl_pred A := 
+  [pred i | p i ==> q i].
+
+Definition eq_simpl_pred {A} (x y : simpl_pred A) := 
+  `=1` x y.
+  
+Instance implP_Proper {A} : Proper (`=1` ==> `=1` ==> eq_simpl_pred) (@predA A).
+Proof.
+  intros f g Hfg f' g' Hfg' i; rewrite /predA /=.
+  now rewrite Hfg Hfg'.
+Qed.
+  
+Lemma on_free_vars_implP p q t : 
+  predA p q =1 xpredT ->
+  on_free_vars p t -> on_free_vars q t.
+Proof.
+  rewrite /predA /=. intros Hp.
+  eapply on_free_vars_impl.
+  intros i hp. specialize (Hp i). now rewrite /= hp in Hp.
+Qed.
+
+Definition shiftnP_predU n p q : 
+  shiftnP n (predU p q) =1 predU (shiftnP n p) (shiftnP n q).
+Proof.
+  intros i.
+  rewrite /shiftnP /predU /=.
+  repeat nat_compare_specs => //.
+Qed.
+
+Instance orP_Proper {A} : Proper (`=1` ==> `=1` ==> eq_simpl_pred) (@predU A).
+Proof.
+  intros f g Hfg f' g' Hfg' i; rewrite /predU /=.
+  now rewrite Hfg Hfg'.
+Qed.
+
+Instance andP_Proper A : Proper (`=1` ==> `=1` ==> eq_simpl_pred) (@predI A).
+Proof.
+  intros f g Hfg f' g' Hfg' i; rewrite /predI /=.
+  now rewrite Hfg Hfg'.
+Qed.
+
+Instance pred_of_simpl_proper {A} : Proper (eq_simpl_pred ==> `=1`) (@PredOfSimpl.coerce A).
+Proof.
+  now move=> f g; rewrite /eq_simpl_pred => Hfg.
+Qed.
+
+Lemma orPL (p q : pred nat) : (predA p (predU p q)) =1 predT.
+Proof.
+  intros i. rewrite /predA /predU /=.
+  rewrite (ssrbool.implybE (p i)).
+  destruct (p i) => //.
+Qed.
+
+
+Lemma orPR (p q : nat -> bool) i : q i -> (predU p q) i.
+Proof.
+  rewrite /predU /= => ->; rewrite orb_true_r //.
+Qed.
+
+(** We need a disjunction here as the substitution can be made of 
+    expanded lets (properly lifted) or just the variables of 
+    [ctx] (lifted by [k]).
+    
+    The proof could certainly be simplified using a more high-level handling of
+    free-variables predicate, which form a simple classical algebra. 
+    To investigate: does ssr's library support this? *)
+
+Lemma on_free_vars_extended_subst p k ctx :
+  on_free_vars_ctx_k p k ctx ->
+  forallb (on_free_vars 
+    (predU (strengthenP 0 (context_assumptions ctx + k) (shiftnP k p)) 
+      (occ_betweenP k (context_assumptions ctx))))
+    (extended_subst ctx k).
+Proof.
+  rewrite /on_free_vars_ctx_k.
+  induction ctx as [|[na [b|] ty] ctx] in p, k |- *; auto.
+  - simpl. rewrite alli_app /= andb_true_r => /andP [] hctx.
+    rewrite /on_free_vars_decl /test_decl /=; len => /andP [] hty /= hb.
+    specialize (IHctx _ k hctx).
+    rewrite IHctx // andb_true_r.
+    eapply on_free_vars_subst => //.
+    len. erewrite on_free_vars_implP => //; cycle 1.
+    { erewrite on_free_vars_lift; eauto. }
+    now rewrite shiftnP_predU /= shiftnP_strengthenP Nat.add_0_r shiftnP_add /= orPL.
+  - cbn. rewrite alli_app /= andb_true_r => /andP [] hctx.
+    rewrite /on_free_vars_decl /test_decl andb_true_r /= => hty.
+    len in hty.
+    specialize (IHctx p k).
+    rewrite andb_idl.
+    * move => _. rewrite /occ_betweenP. repeat nat_compare_specs => /= //.
+    * specialize (IHctx hctx).
+      rewrite (lift_extended_subst' _ 1).
+      rewrite forallb_map.
+      solve_all.
+      apply on_free_vars_lift0.
+      rewrite addnP_orP.
+      eapply on_free_vars_implP; eauto.
+      intros i. rewrite /predA /predU /=.
+      rewrite /strengthenP /= /addnP /=.
+      repeat nat_compare_specs => /= //.
+      + rewrite /occ_betweenP /implb => /=.
+        repeat nat_compare_specs => /= //.
+      + rewrite /shiftnP /occ_betweenP /=.
+        repeat nat_compare_specs => /= //.
+        rewrite !orb_false_r.
+        replace (i + 1 - S (context_assumptions ctx + k) - k) with
+          (i - (context_assumptions ctx + k) - k) by lia.
+        rewrite implybE. destruct p; auto. 
+Qed.
+
+Lemma on_free_vars_expand_lets_k P Γ n t : 
+  n = context_assumptions Γ ->
+  on_free_vars_ctx P Γ ->
+  on_free_vars (shiftnP #|Γ| P) t ->
+  on_free_vars (shiftnP n P) (expand_lets_k Γ 0 t).
+Proof.
+  intros -> HΓ Ht.
+  rewrite /expand_lets_k /=.
+  eapply on_free_vars_impl; cycle 1.
+  - eapply on_free_vars_subst_gen.
+    1:eapply on_free_vars_extended_subst; eauto.
+    rewrite -> on_free_vars_lift. eauto.
+  - len. rewrite /substP /= /strengthenP /=.
+    intros i. simpl. rewrite /shiftnP.
+    repeat nat_compare_specs => /= //.
+    rewrite Nat.sub_0_r. rewrite /orP.
+    replace (i + #|Γ| - context_assumptions Γ - #|Γ|) with (i - context_assumptions Γ) by lia.
+    rewrite /occ_betweenP. repeat nat_compare_specs => /= //.
+    rewrite orb_false_r Nat.sub_0_r.
+    now rewrite orb_diag.
+Qed.
+
+Lemma on_free_vars_terms_inds P ind puinst bodies : 
+  on_free_vars_terms P (inds ind puinst bodies).
+Proof.
+  rewrite /inds.
+  induction #|bodies|; simpl; auto.
+Qed.
+
+Lemma on_free_vars_decl_map P f d :
+  (forall i, on_free_vars P i = on_free_vars P (f i)) ->
+  on_free_vars_decl P d = on_free_vars_decl P (map_decl f d).
+Proof.
+  intros Hi.
+  rewrite /on_free_vars_decl /test_decl.
+  rewrite Hi. f_equal.
+  simpl. destruct (decl_body d) => //.
+  now rewrite /foroptb /= (Hi t).
+Qed.
+
+Lemma on_free_vars_subst_instance_context P u Γ :
+  on_free_vars_ctx P (subst_instance_context u Γ) = on_free_vars_ctx P Γ.
+Proof.
+  rewrite /on_free_vars_ctx.
+  rewrite /subst_instance_context -map_rev alli_map.
+  apply alli_ext => i d.
+  symmetry. apply on_free_vars_decl_map.
+  intros. apply on_free_vars_subst_instance.
+Qed.
+
+Lemma on_free_vars_map2_cstr_args p bctx ctx :
+  #|bctx| = #|ctx| ->
+  on_free_vars_ctx p ctx =
+  on_free_vars_ctx p (map2 set_binder_name bctx ctx).
+Proof.
+  rewrite /on_free_vars_ctx.
+  induction ctx as [|d ctx] in bctx |- *; simpl; auto.
+  - destruct bctx; reflexivity.
+  - destruct bctx => /= //.
+    intros [= hlen].
+    rewrite alli_app (IHctx bctx) // alli_app. f_equal.
+    len. rewrite map2_length // hlen. f_equal.
+Qed.
+
+Lemma on_free_vars_case_branch_context {cf} {Σ} {wfΣ : wf Σ} {P ci i mdecl idecl p br cdecl} :
+  let brctx := case_branch_context ci mdecl p (bcontext br) cdecl in
+  declared_constructor Σ (ci, i) mdecl idecl cdecl ->
+  wf_predicate mdecl idecl p ->
+  wf_branch cdecl br ->
+  forallb (on_free_vars P) (pparams p) ->
+  on_free_vars_ctx P brctx.
+Proof.
+  intros brctx decli wfp wfb havp.
+  rewrite /brctx /case_branch_context /case_branch_context_gen.
+  rewrite (on_free_vars_ctx_all_term _ _ Universe.type0).
+  rewrite -(subst_it_mkProd_or_LetIn _ _ _ (tSort _)).
+  apply on_free_vars_subst => //.
+  rewrite -(expand_lets_it_mkProd_or_LetIn _ _ 0 (tSort _)).
+  eapply on_free_vars_expand_lets_k; len.
+  * rewrite (wf_predicate_length_pars wfp).
+    apply (declared_minductive_ind_npars decli).
+  * eapply closed_ctx_on_free_vars.
+    rewrite closedn_subst_instance_context.
+    apply (declared_inductive_closed_params decli).
+  * rewrite -(subst_it_mkProd_or_LetIn _ _ _ (tSort _)).
+    eapply on_free_vars_impl; cycle 1.
+    + eapply (on_free_vars_subst_gen _ P).
+      { eapply on_free_vars_terms_inds. }
+      rewrite -on_free_vars_ctx_all_term.
+      rewrite on_free_vars_subst_instance_context.
+      rewrite -on_free_vars_map2_cstr_args.
+      { apply (wf_branch_length wfb). }
+      instantiate (1 := closedP (#|mdecl.(ind_bodies)| + #|mdecl.(ind_params)|) xpredT).
+      eapply closedn_ctx_on_free_vars.
+      now move/andP: (declared_constructor_closed wfΣ decli) => [] /andP [].
+    + intros i'.
+      rewrite /substP /= /closedP /shiftnP. len.
+      now repeat nat_compare_specs => /= //.
+Qed.
+
+Lemma on_free_vars_to_extended_list P ctx : 
+  forallb (on_free_vars (shiftnP #|ctx| P)) (to_extended_list ctx).
+Proof.
+  rewrite /to_extended_list /to_extended_list_k.
+  change #|ctx| with (0 + #|ctx|).
+  have: (forallb (on_free_vars (shiftnP (0 + #|ctx|) P)) []) by easy.
+  generalize (@nil term), 0.
+  induction ctx; intros l n.
+  - simpl; auto.
+  - simpl. intros Hl.
+    destruct a as [? [?|] ?].
+    * rewrite Nat.add_succ_r in Hl.
+      specialize (IHctx _ (S n) Hl).
+      now rewrite Nat.add_succ_r Nat.add_1_r.
+    * rewrite Nat.add_succ_r Nat.add_1_r. eapply (IHctx _ (S n)).
+      rewrite -[_ + _](Nat.add_succ_r n #|ctx|) /= Hl.
+      rewrite /shiftnP.
+      nat_compare_specs => /= //.
+Qed.
+
+(** This is less precise than the strengthenP lemma above *)
+Lemma on_free_vars_lift_impl (p : nat -> bool) (n k : nat) (t : term) :
+  on_free_vars (shiftnP k p) t ->
+  on_free_vars (shiftnP (n + k) p) (lift n k t).
+Proof.
+  rewrite -(on_free_vars_lift _ n k t).
+  eapply on_free_vars_impl.
+  intros i.
+  rewrite /shiftnP /strengthenP.
+  repeat nat_compare_specs => /= //.
+  now replace (i - n - k) with (i - (n + k)) by lia.
+Qed.
+
+Lemma on_free_vars_case_predicate_context {cf} {Σ} {wfΣ : wf Σ} {P ci mdecl idecl p} :
+  let pctx := case_predicate_context ci mdecl idecl p in
+  declared_inductive Σ ci mdecl idecl ->
+  wf_predicate mdecl idecl p ->
+  forallb (on_free_vars P) (pparams p) ->
+  on_free_vars (shiftnP #|pcontext p| P) (preturn p) ->
+  on_free_vars_ctx P pctx.
+Proof.
+  intros pctx decli wfp wfb havp.
+  rewrite /pctx /case_predicate_context /case_predicate_context_gen.
+  set (ibinder := {| decl_name := _ |}).
+  rewrite -on_free_vars_map2_cstr_args /=; len.
+  { eapply (wf_predicate_length_pcontext wfp). }
+  rewrite alli_app; len; rewrite andb_true_r.
+  apply andb_true_iff. split.
+  - rewrite -/(on_free_vars_ctx P _).
+    rewrite (on_free_vars_ctx_all_term _ _ Universe.type0).
+    rewrite -(subst_it_mkProd_or_LetIn _ _ _ (tSort _)).
+    apply on_free_vars_subst => //.
+    rewrite -on_free_vars_ctx_all_term.
+    rewrite on_free_vars_subst_instance_context.
+    rewrite (on_free_vars_ctx_all_term _ _ (Universe.type0)).
+    rewrite -(expand_lets_it_mkProd_or_LetIn _ _ 0 (tSort _)).
+    eapply on_free_vars_expand_lets_k; len.
+    * rewrite (wf_predicate_length_pars wfp).
+      apply (declared_minductive_ind_npars decli).
+    * eapply closed_ctx_on_free_vars.
+      apply (declared_inductive_closed_params decli).
+    * eapply on_free_vars_impl; cycle 1.
+      { rewrite <- on_free_vars_ctx_all_term.
+        instantiate (1 := closedP #|mdecl.(ind_params)| xpredT).
+        eapply closedn_ctx_on_free_vars.
+        move: (declared_inductive_closed_pars_indices wfΣ decli).
+        now rewrite closedn_ctx_app => /andP []. }
+       intros i'.
+      rewrite /substP /= /closedP /shiftnP. len.
+      now repeat nat_compare_specs => /= //.
+  - rewrite /on_free_vars_decl /ibinder /test_decl /= /foroptb /= andb_true_r.
+    rewrite on_free_vars_mkApps /= forallb_app /=.
+    rewrite on_free_vars_to_extended_list /= andb_true_r.
+    rewrite -/(is_true _).
+    rewrite forallb_map. unshelve eapply (forallb_impl _ _ _ _ wfb).
+    intros. simpl.
+    eapply on_free_vars_lift0. now rewrite addnP_shiftnP.
+Qed.
+
+Lemma foron_free_vars_extended_subst brctx p :
+  on_free_vars_ctx p brctx ->
+  forallb (on_free_vars (shiftnP (context_assumptions brctx) p))
+    (extended_subst brctx 0).
+Proof.
+  move/on_free_vars_extended_subst.
+  eapply forallb_impl.
+  intros x hin.
+  rewrite Nat.add_0_r shiftnP0.
+  eapply on_free_vars_impl.
+  intros i. rewrite /orP /strengthenP /= /occ_betweenP /shiftnP.
+  repeat nat_compare_specs => /= //.
+  now rewrite orb_false_r.
+Qed.
+
+Lemma on_free_vars_fix_subst P mfix idx :
+  on_free_vars P (tFix mfix idx) ->
+  forallb (on_free_vars P) (fix_subst mfix).
+Proof.
+  move=> /=; rewrite /fix_subst.
+  intros hmfix. generalize hmfix.
+  induction mfix at 2 4; simpl; auto.
+  move/andP => [ha hm]. rewrite IHm // andb_true_r //.
+Qed.
+
+Lemma on_free_vars_unfold_fix P mfix idx narg fn :
+  unfold_fix mfix idx = Some (narg, fn) ->
+  on_free_vars P (tFix mfix idx) ->
+  on_free_vars P fn.
+Proof.
+  rewrite /unfold_fix. 
+  destruct nth_error eqn:hnth => // [=] _ <- /=.
+  intros hmfix; generalize hmfix.
+  move/forallb_All/(nth_error_all hnth) => /andP [] _ Hbody.
+  eapply on_free_vars_subst; len => //.
+  eapply (on_free_vars_fix_subst _ _ idx) => //.
+Qed.
+
+Lemma on_free_vars_cofix_subst P mfix idx :
+  on_free_vars P (tCoFix mfix idx) ->
+  forallb (on_free_vars P) (cofix_subst mfix).
+Proof.
+  move=> /=; rewrite /cofix_subst.
+  intros hmfix. generalize hmfix.
+  induction mfix at 2 4; simpl; auto.
+  move/andP => [ha hm]. rewrite IHm // andb_true_r //.
+Qed.
+
+Lemma on_free_vars_unfold_cofix P mfix idx narg fn :
+  unfold_cofix mfix idx = Some (narg, fn) ->
+  on_free_vars P (tCoFix mfix idx) ->
+  on_free_vars P fn.
+Proof.
+  rewrite /unfold_cofix. 
+  destruct nth_error eqn:hnth => // [=] _ <- /=.
+  intros hmfix; generalize hmfix.
+  move/forallb_All/(nth_error_all hnth) => /andP [] _ Hbody.
+  eapply on_free_vars_subst; len => //.
+  eapply (on_free_vars_cofix_subst _ _ idx) => //.
+Qed.
+
+Lemma addnP_shiftnP_comm n (P : nat -> bool) : P 0 -> addnP 1 (shiftnP n P) =1 shiftnP n (addnP 1 P).
+Proof.
+  intros p0 i; rewrite /addnP /shiftnP /=.
+  repeat nat_compare_specs => /= //. 
+  - assert (n = i + 1) as -> by lia.
+    now replace (i + 1 - (i + 1)) with 0 by lia.
+  - lia_f_equal.
+Qed.
+
+Lemma on_ctx_free_vars_concat P Γ Δ : 
+  on_ctx_free_vars P Γ ->
+  on_ctx_free_vars (shiftnP #|Δ| P) Δ ->  
+  on_ctx_free_vars (shiftnP #|Δ| P) (Γ ,,, Δ).
+Proof.
+  rewrite /on_ctx_free_vars alli_app.
+  move=> hΓ -> /=; rewrite alli_shiftn.
+  eapply alli_impl; tea => i d /=.
+  simpl.
+  rewrite {1}/shiftnP. nat_compare_specs.
+  replace (#|Δ| + i - #|Δ|) with i by lia.
+  destruct (P i) eqn:pi => /= //.
+  apply on_free_vars_decl_impl => k.
+  rewrite /addnP /shiftnP.
+  nat_compare_specs.
+  now replace (k + S (#|Δ| + i) - #|Δ|) with (k + S i) by lia.
+Qed.
+
+Lemma on_ctx_free_vars_tip P d : on_ctx_free_vars P [d] = P 0 ==> on_free_vars_decl (addnP 1 P) d.
+Proof.
+  now rewrite /on_ctx_free_vars /= /= andb_true_r.
+Qed.
+
+Lemma shiftnPS n P : shiftnP (S n) P n.
+Proof.
+  rewrite /shiftnP /=.
+  now nat_compare_specs.
+Qed.
+
+Lemma on_ctx_free_vars_extend P Γ Δ :
+  on_free_vars_ctx P Δ ->
+  on_ctx_free_vars P Γ ->
+  on_ctx_free_vars (shiftnP #|Δ| P) (Γ ,,, Δ).
+Proof.
+  intros hΔ hΓ.
+  apply on_ctx_free_vars_concat => //.
+  revert P Γ hΓ hΔ.
+  induction Δ using rev_ind; simpl; auto; intros P Γ hΓ.
+  rewrite /on_ctx_free_vars /on_free_vars_ctx List.rev_app_distr /= shiftnP0.
+  rewrite alli_shift. setoid_rewrite Nat.add_comm. setoid_rewrite <- shiftnP_add.
+  move/andP=> [] hx hΔ.
+  rewrite alli_app /= andb_true_r Nat.add_0_r; len.
+  rewrite Nat.add_comm.
+  rewrite addnP_shiftnP.
+  specialize (IHΔ (shiftnP 1 P) (Γ ,, x)).
+  forward IHΔ.
+  * simpl. apply (on_ctx_free_vars_concat _ _ [x]) => //.
+    simpl.
+    now rewrite on_ctx_free_vars_tip {1}/shiftnP /= addnP_shiftnP.
+  * specialize (IHΔ hΔ).
+    rewrite shiftnPS /= hx andb_true_r.
+    rewrite /on_ctx_free_vars in IHΔ.
+    rewrite -(Nat.add_1_r #|Δ|).
+    setoid_rewrite <-(shiftnP_add).
+    now setoid_rewrite <- (shiftnP_add _ _ _ _).
+Qed.
+
+Lemma on_free_vars_fix_context P mfix : 
+  All (fun x : def term =>
+      test_def (on_free_vars P) (on_free_vars (shiftnP #|mfix| P)) x)
+      mfix ->
+  on_free_vars_ctx P (fix_context mfix).
+Proof.
+  intros a.
+  assert (All (fun x => on_free_vars P x.(dtype)) mfix).
+  { solve_all. now move/andP: H=> []. } clear a.
+  induction mfix using rev_ind; simpl; auto.
+  rewrite /fix_context /= mapi_app List.rev_app_distr /=.
+  rewrite /on_free_vars_ctx /= alli_app. len.
+  rewrite andb_true_r.
+  eapply All_app in X as [X Hx].
+  depelim Hx. clear Hx.
+  specialize (IHmfix X).
+  rewrite /on_free_vars_ctx in IHmfix.
+  rewrite IHmfix /= /on_free_vars_decl /test_decl /= /foroptb /= andb_true_r.
+  apply on_free_vars_lift0.
+  now rewrite addnP_shiftnP.
+Qed.
+
+(** This shows preservation by reduction of closed/noccur_between predicates 
+  necessary to prove exchange and strengthening lemmas. *)
+Lemma red1_on_free_vars {cf} {P : nat -> bool} {Σ Γ u v} {wfΣ : wf Σ} :
+  on_free_vars P u ->
+  on_ctx_free_vars P Γ ->
+  red1 Σ Γ u v ->
+  on_free_vars P v.
+Proof.
+  intros hav hctx h.
+  induction h using red1_ind_all in P, hav, hctx |- *.
+  all: try solve [
+    simpl ; constructor ; eapply IHh ;
+    try (simpl in hav; rtoProp);
+    try eapply urenaming_vass ;
+    try eapply urenaming_vdef ;
+    assumption
+  ].
+  all:simpl in hav |- *; try toAll.
+  all:try move/and3P: hav => [h1 h2 h3].
+  all:try (move/andP: hav => [] /andP [] h1 h2 h3).
+  all:try move/andP: hav => [h1 h2].
+  all:try move/andP: h3 => [] h3 h4.
+  all:try rewrite ?h1 // ?h2 // ?h3 // ?h4 // ?IHh /= // ?andb_true_r.
+  all:try eapply on_free_vars_subst1; eauto.
+  - destruct (nth_error Γ i) eqn:hnth => //.
+    simpl in H. noconf H.
+    epose proof (nth_error_on_free_vars_ctx P 0 Γ i c).
+    forward H0. { now rewrite addnP0. }
+    specialize (H0 hav hnth). simpl in H0.
+    rewrite /test_decl H in H0.
+    rewrite on_free_vars_lift0 //.
+    move/andP: H0 => [].
+    now rewrite /foroptb /= => _ hbod.
+  - rewrite /iota_red. rename h4 into hbrs.
+    move: h3. rewrite on_free_vars_mkApps => /andP [] hf hargs.
+    apply on_free_vars_subst.
+    { rewrite forallb_skipn //. }
+    rewrite H2.
+    rewrite /expand_lets /expand_lets_k /=.
+    eapply on_free_vars_subst.
+    * eapply foron_free_vars_extended_subst.
+      eapply on_free_vars_case_branch_context; eauto.
+    * rewrite extended_subst_length.
+      rewrite (case_branch_context_length H1).
+      rewrite shiftnP_add.
+      eapply nth_error_forallb in hbrs; eauto.
+      simpl in hbrs.
+      eapply on_free_vars_lift_impl in hbrs.
+      now rewrite Nat.add_comm.
+  - rewrite !on_free_vars_mkApps in hav |- *.
+    rtoProp.
+    eapply on_free_vars_unfold_fix in H; eauto. 
+  - move: h3; rewrite !on_free_vars_mkApps.
+    move=> /andP[] hcofix ->.
+    eapply on_free_vars_unfold_cofix in hcofix; eauto.
+    now rewrite hcofix.
+  - move: hav; rewrite !on_free_vars_mkApps => /andP [] hcofix ->.
+    eapply on_free_vars_unfold_cofix in H as ->; eauto.
+  - eapply closed_on_free_vars. rewrite closedn_subst_instance_constr.
+    eapply declared_constant_closed_body; eauto.
+  - move: hav; rewrite on_free_vars_mkApps /=.
+    now move/(nth_error_forallb H).
+  - rewrite (on_ctx_free_vars_concat _ _ [_]) // /=
+      on_ctx_free_vars_tip /= addnP_shiftnP /on_free_vars_decl
+      /test_decl /= andb_true_r //.
+  - rewrite (on_ctx_free_vars_concat _ _ [_]) //
+      on_ctx_free_vars_tip /= addnP_shiftnP /on_free_vars_decl /test_decl /= h2 /=
+      /foroptb /= h1 //.
+  - solve_all.
+    eapply OnOne2_impl_All_r; eauto. solve_all.
+  - rewrite /pctx.
+    rewrite -(case_predicate_context_length (ci:=ci) H).
+    eapply on_ctx_free_vars_extend => //.
+    apply (on_free_vars_case_predicate_context isdecl H h1 h2).
+  - toAll.
+    eapply Forall2_All2 in H0.
+    eapply OnOne2All_All2_mix_left in X; eauto.
+    eapply OnOne2All_nth_error_impl in X.
+    eapply OnOne2All_impl_All_r in X; eauto; solve_all.
+    destruct a as [cidx hnth].
+    rewrite -b. eapply b1 => //.
+    erewrite <- (case_branch_context_length b0).
+    eapply on_ctx_free_vars_extend => //.
+    eapply (on_free_vars_case_branch_context (i := cidx)); eauto.
+    * split; eauto.
+    * solve_all.
+  - rewrite (on_ctx_free_vars_concat _ _ [_]) // /=
+      on_ctx_free_vars_tip /= addnP_shiftnP /on_free_vars_decl /test_decl /= h1 /= //.
+  - toAll. eapply OnOne2_impl_All_r; eauto; solve_all.
+  - toAll. unfold test_def.
+    rewrite -(OnOne2_length X).
+    eapply OnOne2_impl_All_r; eauto; solve_all.
+    destruct x, y; noconf b; simpl in *. rtoProp; solve_all.
+  - toAll. unfold test_def in *. rewrite -(OnOne2_length X).
+    eapply OnOne2_impl_All_r; eauto; solve_all.
+    destruct x, y; noconf b; simpl in *; rtoProp; solve_all.
+    apply b0 => //.
+    rewrite -(fix_context_length mfix0).
+    eapply on_ctx_free_vars_extend => //.
+    now apply on_free_vars_fix_context.
+  - toAll. unfold test_def.
+    rewrite -(OnOne2_length X).
+    eapply OnOne2_impl_All_r; eauto; solve_all.
+    destruct x, y; noconf b; simpl in *. rtoProp; solve_all.
+  - toAll. unfold test_def in *. rewrite -(OnOne2_length X).
+    eapply OnOne2_impl_All_r; eauto; solve_all.
+    destruct x, y; noconf b; simpl in *; rtoProp; solve_all.
+    apply b0 => //.
+    rewrite -(fix_context_length mfix0).
+    eapply on_ctx_free_vars_extend => //.
+    now apply on_free_vars_fix_context.
+Qed.
+
+(*
+Lemma typing_on_free_vars : env_prop
+  (fun Σ Γ t A =>
+    forall P,
+    on_free_vars (closedP #|Γ| P) t ->
+    ∑ Af, (red Σ Γ A Af * on_free_vars (closedP #|Γ| P) Af))
+   (fun Σ Γ =>
+   All_local_env
+   (lift_typing (fun (Σ : global_env_ext) (Γ : context) (t T : term)
+    =>
+    forall P,
+    on_free_vars (closedP #|Γ| P) t ->
+    ∑ Af, (red1 Σ Γ T Af * on_free_vars (closedP #|Γ| P) Af)) Σ) Γ).
+Proof.
+  
+  apply typing_ind_env.
+  7:{
+    - intros Σ wfΣ Γ wfΓ t na A B a u X hty ihty ht iht hu ihu P.
+      simpl. move/andP=> [havt havs].
+      destruct (iht _ havt) as [ty [redty hav]].
+      eapply invert_red_prod in redty as [A' [B' [[eq redA] redB]]]. subst ty.
+      move: hav => /= /andP [hA' hB'].
+      eexists (B' {0 := a}); split. 1:admit.
+      eapply on_free_vars_subst=> /=; rewrite ?havs //. }
+  2:{ - intros Σ wfΣ Γ wfΓ n decl isdecl ihΓ P.
+        simpl in * => hn.
+        eexists; split; eauto.
+        eapply (nth_error_All_local_env (n:=n)) in ihΓ.
+        2:{ eapply nth_error_Some_length in isdecl; eauto. }
+        rewrite isdecl in ihΓ. simpl in ihΓ. rewrite /closedP in hn.
+        move: hn; nat_compare_specs => //. intros pn.
+        move: ihΓ. unfold on_local_decl. 
+        destruct decl_body eqn:db;
+        unfold lift_typing; simpl.
+        * intros ih. specialize (ih P).
+          rewrite skipn_length // in ih.
+          rewrite on_free_vars_lift0 //.
+          admit.
+        * admit. }
+
+  13:{
+    - intros Σ wfΣ Γ wfΓ t A B X hwf ht iht htB ihB cum P hav.
+      specialize (iht _ hav) as [Af [redAf havaf]].
+      admit. (* certainly provable *)
+  }
+Admitted.*)
+
+(* 
+Lemma typing_rename_prop' : env_prop
+  (fun Σ Γ t A =>
+    forall Δ f,
+    renaming (closedP #|Γ| xpredT) Σ Δ Γ f ->
+    Σ ;;; Δ |- rename f t : rename f A)
+   (fun Σ Γ =>
+   All_local_env
+   (lift_typing (fun (Σ : global_env_ext) (Γ : context) (t T : term)
+    =>
+    forall P (Δ : PCUICEnvironment.context) (f : nat -> nat),
+    renaming (closedP #|Γ| P) Σ Δ Γ f -> 
+    Σ;;; Δ |- rename f t : rename f T) Σ) Γ).
+Proof.
+  red. intros.
+  destruct (typing_rename_prop Σ wfΣ Γ t T ty) as [? []].
+  split.
+  - eapply on_global_env_impl. 2:eapply f.
+    intros.
+    red in X0. destruct T0; red.
+    * intros.
+      eapply (X0 xpredT).
+      
+
+
+  destruct X. *)
